New TLUL spec

cava2/TLUL.v
@@ -17,6 +17,8 @@
 Require Import Coq.Lists.List.
 Require Import Coq.ZArith.ZArith.
 
+Import ListNotations.
+
 Require Import Cava.Expr.
 Require Import Cava.ExprProperties.
 Require Import Cava.Invariant.
@@ -351,28 +353,28 @@ Section TLULSpec.
   | OutstandingGet (reqid : N) (reqsz : N)
   | OutstandingPutFullData (reqid : N).
 
-  Definition tlul_repr := option TLULState.
 
-  Compute denote_type (input_of tlul_adapter_reg).
+  Fixpoint outstanding_h2d (inputs : list tl_h2d) :=
+    match inputs with
+    | [] => None
+    | h :: tl =>
+      match outstanding_h2d tl with
+      | None => if a_valid h then Some h else None
+      | Some h' => if d_ready h then None else Some h'
+      end
+    end.
+
+  Definition tlul_repr := list tl_h2d.
+
   Instance tlul_specification
     : specification_for (tlul_adapter_reg (reg_count:=reg_count)) tlul_repr :=
-    {| reset_repr := None;
+    {| reset_repr := [];
 
        update_repr :=
          fun (input : denote_type (input_of (tlul_adapter_reg (reg_count:=reg_count))))
            (repr : tlul_repr) =>
            let '(h2d, (_regs, tt)) := input in
-           match repr with
-           | None =>
-             if a_valid h2d then
-               if a_opcode h2d =? Get then
-                 Some (OutstandingGet (a_source h2d) (a_size h2d))
-               else if a_opcode h2d =? PutFullData then
-                      Some (OutstandingPutFullData (a_source h2d))
-                    else (* unrechable *) repr
-             else None
-           | Some _ => if d_ready h2d then None else repr
-           end;
+           h2d :: repr;
 
        precondition :=
          fun (input : denote_type (input_of tlul_adapter_reg))
@@ -386,22 +388,11 @@ Section TLULSpec.
          fun (input : denote_type (input_of (tlul_adapter_reg (reg_count:=reg_count))))
            (repr : tlul_repr)
            (output : denote_type (output_of (tlul_adapter_reg (reg_count:=reg_count)))) =>
-           exists h2d regs d2h io_re io_we io_address io_data io_mask repr',
+           exists h2d regs d2h io_re io_we io_address io_data io_mask,
                input = (h2d, (regs, tt))
-               /\ repr' =
-                  match repr with
-                  | None =>
-                    if a_valid h2d then
-                      if a_opcode h2d =? Get then
-                        Some (OutstandingGet (a_source h2d) (a_size h2d))
-                      else if a_opcode h2d =? PutFullData then
-                             Some (OutstandingPutFullData (a_source h2d))
-                           else (* unrechable *) repr
-                    else None
-                  | Some _ => if d_ready h2d then None else repr
-                  end
                /\ output = (d2h, (io_re, (io_we, (io_address, (io_data, io_mask)))))
-               /\ match repr' with
+
+               /\ match outstanding_h2d (h2d :: repr) with
                  | None =>
                    d_valid    d2h = false
                    /\ d_param  d2h = 0
@@ -412,64 +403,67 @@ Section TLULSpec.
                    /\ io_re = false
                    /\ io_we = false
 
-                 | Some (OutstandingGet reqid reqsz) =>
-                   d_valid    d2h = true
-                   /\ d_opcode d2h = AccessAckData
-                   /\ d_param  d2h = 0
-                   /\ d_size   d2h = reqsz
-                   /\ d_source d2h = reqid
-                   /\ d_sink   d2h = 0
-                   /\ d_data   d2h = List.nth (N.to_nat (((a_address h2d / 4) mod (2 ^ 30)))) regs 0%N
-                   /\ d_user   d2h = 0
-                   /\ d_error  d2h = false
-                   /\ a_ready  d2h = false
-                   /\ match repr with
-                     | None => if a_valid h2d then
-                                io_re = true
-                                /\ io_address = a_address h2d
-                              else True
-                     | _ => True
-                     end
-                   /\ io_we = false
-
-                 | Some (OutstandingPutFullData reqid) =>
-                   d_valid    d2h = true
-                   /\ d_opcode d2h = AccessAck
-                   /\ d_param  d2h = 0
-                   (* /\ d_size   d2h =  *)
-                   /\ d_source d2h = reqid
-                   /\ d_sink   d2h = 0
-                   /\ d_user   d2h = 0
-                   /\ d_error  d2h = false
-                   /\ a_ready  d2h = false
-                   /\ io_re = false
-                   /\ match repr with
-                     | None => if a_valid h2d then
-                                io_we = true
-                                /\ io_address = a_address h2d
-                                /\ io_data = a_data h2d
-                                /\ io_mask = a_mask h2d
-                              else True
-                     | _ => True
-                     end
+                 | Some h2d' =>
+                   if a_opcode h2d' =? Get then
+                     d_valid    d2h = true
+                     /\ d_opcode d2h = AccessAckData
+                     /\ d_param  d2h = 0
+                     /\ d_size   d2h = a_size h2d'
+                     /\ d_source d2h = a_source h2d'
+                     /\ d_sink   d2h = 0
+                     /\ d_data   d2h = List.nth (N.to_nat (((a_address h2d / 4) mod (2 ^ 30)))) regs 0%N
+                     /\ d_user   d2h = 0
+                     /\ d_error  d2h = false
+                     /\ a_ready  d2h = false
+                     /\ match outstanding_h2d repr with
+                       | None => if a_valid h2d then
+                                  io_re = true
+                                  /\ io_address = a_address h2d
+                                else True
+                       | _ => True
+                       end
+                     /\ io_we = false
+                   else if a_opcode h2d' =? PutFullData then
+                          d_valid    d2h = true
+                          /\ d_opcode d2h = AccessAck
+                          /\ d_param  d2h = 0
+                          (* /\ d_size   d2h =  *)
+                          /\ d_source d2h = a_source h2d'
+                          /\ d_sink   d2h = 0
+                          /\ d_user   d2h = 0
+                          /\ d_error  d2h = false
+                          /\ a_ready  d2h = false
+                          /\ io_re = false
+                          /\ match outstanding_h2d repr with
+                            | None => if a_valid h2d then
+                                       io_we = true
+                                       /\ io_address = a_address h2d
+                                       /\ io_data = a_data h2d
+                                       /\ io_mask = a_mask h2d
+                                     else True
+                            | _ => True
+                            end
+                        else True
                  end
     |}.
 
   Global Instance tlul_invariant : invariant_for (tlul_adapter_reg (reg_count:=reg_count)) tlul_repr :=
     fun (state : denote_type (state_of tlul_adapter_reg)) repr =>
       tlul_adapter_reg_state_error state = false
-      /\ match repr with
+      /\ match outstanding_h2d repr with
         | None =>
           tlul_adapter_reg_state_outstanding (reg_count:=reg_count) state = false
-        | Some (OutstandingGet reqid reqsz) =>
-          tlul_adapter_reg_state_outstanding state = true
-          /\ tlul_adapter_reg_state_reqid state = reqid
-          /\ tlul_adapter_reg_state_reqsz state = reqsz
-          /\ tlul_adapter_reg_state_rspop state = AccessAckData
-        | Some (OutstandingPutFullData reqid) =>
-          tlul_adapter_reg_state_outstanding state = true
-          /\ tlul_adapter_reg_state_reqid state = reqid
-          /\ tlul_adapter_reg_state_rspop state = AccessAck
+        | Some h2d =>
+          if a_opcode h2d =? Get then
+            tlul_adapter_reg_state_outstanding state = true
+            /\ tlul_adapter_reg_state_reqid state = a_source h2d
+            /\ tlul_adapter_reg_state_reqsz state = a_size h2d
+            /\ tlul_adapter_reg_state_rspop state = AccessAckData
+          else if a_opcode h2d =? PutFullData then
+                 tlul_adapter_reg_state_outstanding state = true
+                 /\ tlul_adapter_reg_state_reqid state = a_source h2d
+                 /\ tlul_adapter_reg_state_rspop state = AccessAck
+               else False
         end.
 
     Lemma tlul_adapter_reg_invariant_at_reset : invariant_at_reset tlul_adapter_reg.
@@ -488,24 +482,65 @@ Section TLULSpec.
       intros; subst.
       simplify_invariant (tlul_adapter_reg (reg_count:=reg_count)).
       simplify_spec (tlul_adapter_reg (reg_count:=reg_count)).
-      cbv [tlul_adapter_reg]. stepsimpl. logical_simplify.
+      cbv [tlul_adapter_reg].
+      stepsimpl.
       tlul_adapter_reg_state_simpl. tlsimpl.
+      logical_simplify.
       match goal with
       | h : reg_count = _ |- _ => clear h
       end.
       repeat (destruct_pair_let; cbn [fst snd]).
-      destruct repr as [[|]|]; [| |].
-      1-2: (* repr = Some _ *)
-        logical_simplify; subst;
-        tlul_adapter_reg_state_simpl; boolsimpl; cbn [fst snd];
-          destruct d_ready0; ssplit; reflexivity.
-      (* repr = None *)
-      subst. tlul_adapter_reg_state_simpl. boolsimpl.
-      destruct a_valid0;
-        try match goal with
-            | h: true = true -> _ |- _ => destruct h; subst
-            end;
-        cbn; ssplit; reflexivity.
+      tlul_adapter_reg_state_simpl.
+      split.
+      - destruct (a_valid0 && negb outstanding)%bool; subst; reflexivity.
+      - remember (outstanding_h2d
+                    ((a_valid0,
+                      (a_opcode0,
+                       (a_param0, (a_size0, (a_source0, (a_address0, (a_mask0, (a_data0, (a_user0, d_ready0))))))))) :: repr)) as outs eqn:Eouts.
+        destruct outs; subst.
+        + simpl in Eouts.
+          remember (outstanding_h2d repr) as outs' eqn:Eouts'.
+          destruct outs'; subst.
+          * destruct d_ready0; subst.
+            -- discriminate Eouts.
+            -- inversion Eouts; subst; clear Eouts.
+               destruct (a_opcode t0 =? Get).
+               ++ logical_simplify. subst. boolsimpl.
+                  ssplit; reflexivity.
+               ++ destruct (a_opcode t0 =? PutFullData).
+                  ** logical_simplify. subst. boolsimpl.
+                     ssplit; reflexivity.
+                  ** auto.
+          * destruct a_valid0.
+            -- inversion Eouts; subst; clear Eouts.
+               cbn.
+               destruct (a_opcode0 =? Get) eqn:Hget.
+               ++ ssplit; reflexivity.
+               ++ destruct (a_opcode0 =? PutFullData) eqn:Hput.
+                  ** ssplit; reflexivity.
+                  ** apply N.eqb_neq in Hget, Hput.
+                     destruct H1.
+                     --- reflexivity.
+                     --- apply Hget. assumption.
+                     --- apply Hput. assumption.
+            -- discriminate Eouts.
+        + simpl in Eouts.
+          remember (outstanding_h2d repr) as outs' eqn:Eouts'.
+          destruct outs'; subst.
+          -- destruct (a_opcode t =? Get) eqn:Hget.
+             ++ logical_simplify; subst. boolsimpl.
+                destruct d_ready0.
+                ** reflexivity.
+                ** discriminate Eouts.
+             ++ destruct (a_opcode t =? PutFullData) eqn:Hput.
+                ** logical_simplify; subst. boolsimpl.
+                   destruct d_ready0.
+                   --- reflexivity.
+                   --- discriminate Eouts.
+                ** inversion H2.
+          -- destruct a_valid0.
+             +++ discriminate Eouts.
+             +++ boolsimpl. reflexivity.
     Qed.
 
     Lemma tlul_adapter_reg_output_correct : output_correct tlul_adapter_reg.
@@ -525,31 +560,85 @@ Section TLULSpec.
       end.
       subst.
       repeat (destruct_pair_let; cbn [fst snd]).
-      destruct repr as [repr'|].
-      - (* repr = Some _ *)
-        destruct repr'; logical_simplify; subst; boolsimpl;
-          eexists _, _, _, _, _, _, _, _, _;
-          cbn -[N.ones]; repeat (rewrite pair_equal_spec);
-            tlsimpl; ssplit; try reflexivity;
-              destruct d_ready0; simpl; ssplit; auto; [].
-        rewrite N.land_ones.
-        replace 4 with (2 ^ 2) by reflexivity.
-        rewrite <- ! N.shiftr_div_pow2.
-        reflexivity.
-      - (* repr = None *)
-        subst.
-        eexists _, _, _, _, _, _, _, _, _.
-        cbn -[N.ones]. repeat (rewrite pair_equal_spec).
-        tlsimpl. ssplit; try reflexivity; [].
-        destruct a_valid0; simpl; ssplit; try reflexivity; [].
-        match goal with
-        | h: true = true -> _ |- _ =>
-          destruct h; [reflexivity|..]
-        end; subst; simpl; ssplit; try reflexivity; [].
-        rewrite N.land_ones.
-        replace 4 with (2 ^ 2) by reflexivity.
-        rewrite <- ! N.shiftr_div_pow2.
-        reflexivity.
+      remember (outstanding_h2d
+                  ((a_valid0,
+                    (a_opcode0,
+                     (a_param0, (a_size0, (a_source0, (a_address0, (a_mask0, (a_data0, (a_user0, d_ready0))))))))) :: repr)) as outs eqn:Eouts.
+      destruct outs; subst.
+      - simpl in Eouts.
+        remember (outstanding_h2d repr) as outs' eqn:Eouts'.
+        destruct outs'; subst;
+          destruct d_ready0; try discriminate Eouts; inversion Eouts; subst; clear Eouts.
+        + destruct (a_opcode t0 =? Get) eqn:Hget; logical_simplify; subst; boolsimpl.
+          * do 8 eexists. split. 1: reflexivity.
+            cbn -[N.ones]. split. 1: reflexivity.
+            subst. rewrite <- Eouts'. rewrite Hget. tlsimpl.
+            ssplit; try reflexivity.
+            rewrite N.land_ones.
+            replace 4 with (2 ^ 2) by reflexivity.
+            rewrite <- ! N.shiftr_div_pow2.
+            reflexivity.
+          * destruct (a_opcode t0 =? PutFullData) eqn:Hput; logical_simplify; subst; boolsimpl.
+            -- do 8 eexists. split. 1: reflexivity.
+               cbn -[N.ones]. split. 1: reflexivity.
+               subst. rewrite <- Eouts'. rewrite Hget, Hput. tlsimpl.
+               ssplit; reflexivity.
+            -- inversion H1.
+        + destruct a_valid0; try discriminate H0.
+          inversion H0; subst. clear H0.
+          do 8 eexists. split. 1: reflexivity.
+          cbn -[N.ones]. split. 1: reflexivity.
+          subst. rewrite <- Eouts'. tlsimpl.
+          destruct H2.
+          * reflexivity.
+          * rewrite H. boolsimpl. cbn -[N.ones].
+            ssplit; try reflexivity.
+            rewrite N.land_ones.
+            replace 4 with (2 ^ 2) by reflexivity.
+            rewrite <- ! N.shiftr_div_pow2.
+            reflexivity.
+          * rewrite H. boolsimpl. cbn. ssplit; reflexivity.
+        + destruct a_valid0; try discriminate H0.
+          inversion H0; subst. clear H0.
+          do 8 eexists. split. 1: reflexivity.
+          cbn -[N.ones]. split. 1: reflexivity.
+          subst. rewrite <- Eouts'. tlsimpl.
+          destruct H2.
+          * reflexivity.
+          * rewrite H. boolsimpl. cbn -[N.ones].
+            ssplit; try reflexivity.
+            rewrite N.land_ones.
+            replace 4 with (2 ^ 2) by reflexivity.
+            rewrite <- ! N.shiftr_div_pow2.
+            reflexivity.
+          * rewrite H. boolsimpl. cbn. ssplit; reflexivity.
+      - simpl in Eouts.
+        remember (outstanding_h2d repr) as outs' eqn:Eouts'.
+        destruct outs'; subst;
+          destruct d_ready0; try discriminate Eouts; inversion Eouts; subst; clear Eouts.
+        + destruct (a_opcode t =? Get) eqn:Hget; logical_simplify; subst; boolsimpl.
+          * do 8 eexists. split. 1: reflexivity.
+            cbn -[N.ones]. split. 1: reflexivity.
+            subst. rewrite <- Eouts'. tlsimpl.
+            ssplit; reflexivity.
+          * destruct (a_opcode t =? PutFullData) eqn:Hput; logical_simplify; subst; boolsimpl.
+            -- do 8 eexists. split. 1: reflexivity.
+               cbn -[N.ones]. split. 1: reflexivity.
+               subst. rewrite <- Eouts'. tlsimpl.
+               ssplit; reflexivity.
+            -- inversion H1.
+        + destruct a_valid0; try discriminate H0.
+          clear H0.
+          do 8 eexists. split. 1: reflexivity.
+          cbn -[N.ones]. split. 1: reflexivity.
+          subst. rewrite <- Eouts'. tlsimpl.
+          ssplit; reflexivity.
+        + destruct a_valid0; try discriminate H0.
+          clear H0.
+          do 8 eexists. split. 1: reflexivity.
+          cbn -[N.ones]. split. 1: reflexivity.
+          subst. rewrite <- Eouts'. tlsimpl.
+          ssplit; reflexivity.
     Qed.
 
     Existing Instances tlul_adapter_reg_invariant_at_reset tlul_adapter_reg_invariant_preserved
